import Lib.IntTypes from _dev_inttypes

lib/Lib.IntTypes.fst
@@ -19,7 +19,16 @@ let sec_int_t t = pub_int_t t
 
 let sec_int_v #t u = pub_int_v u
 
-let uintv_extensionality #t #l a b =
+val intv_extensionality:
+   #t:inttype
+ -> #l:secrecy_level
+ -> a:int_t t l
+ -> b:int_t t l
+ -> Lemma
+  (requires int_v #t #l a == int_v #t #l b)
+  (ensures  a == b)
+  
+let intv_extensionality #t #l a b =
   match t with
   | U1   -> ()
   | U8   -> UInt8.v_inj a b
@@ -31,13 +40,16 @@ let uintv_extensionality #t #l a b =
   | S16  -> Int16.v_inj a b
   | S32  -> Int32.v_inj a b
   | S64  -> Int64.v_inj a b
-  //| S128 -> Int128.v_inj a b
+  | S128 -> Int128.v_inj a b
+
 
 (* Declared in .fsti: uint8, uint16, uint32, uint64, uint128 *)
 
 let secret #t x = x
 
-let uint #t #l x =
+#reset-options
+
+let mk_int #t #l x =
   match t with
   | U1 -> UInt8.uint_to_t x
   | U8 -> UInt8.uint_to_t x
@@ -49,16 +61,18 @@ let uint #t #l x =
   | S16 -> Int16.int_to_t x
   | S32 -> Int32.int_to_t x
   | S64 -> Int64.int_to_t x
-  //| S128 -> Int128.int_to_t x
+  | S128 -> Int128.int_to_t x
   
-let uintv_injective #t #l a =
-  uintv_extensionality a (uint (uint_v a))
+  
+let intv_injective #t #l a =
+  intv_extensionality a (mk_int (int_v a))
 
-let u16_us x = x
+(*let u16_us x = x
 let u32_ul x = x
 let u64_uL x = x
+*)
 
-let u128 x = FStar.UInt128.uint64_to_uint128 (u64 x)
+//let u128 x = FStar.UInt128.uint64_to_uint128 (u64 x)
 
 let size_v_size_lemma s = ()
 
@@ -72,7 +86,7 @@ let byte_to_uint8 x = x
 
 let byte_to_int8 x = FStar.Int.Cast.uint8_to_int8 x
 
-let nat_to_uint #t #l x =
+let nat_to_int #t #l x =
   match t with
   | U1 -> u8 x
   | U8 -> u8 x
@@ -84,6 +98,7 @@ let nat_to_uint #t #l x =
   | S16 -> i16 x
   | S32 -> i32 x
   | S64 -> i64 x
+  | S128 -> Int128.int_to_t x
   
 #reset-options "--z3rlimit 500"
 
@@ -99,6 +114,7 @@ let cast #t #l t' l' u  =
   | U1, S16 -> FStar.Int.Cast.uint8_to_int16 u
   | U1, S32 -> FStar.Int.Cast.uint8_to_int32 u
   | U1, S64 -> FStar.Int.Cast.uint8_to_int64 u
+  | U1, S128 -> mk_int #S128 #l' (uint_v u)
   | U8, U1 -> FStar.UInt8.rem u 2uy
   | U8, U8 -> u
   | U8, U16 -> FStar.Int.Cast.uint8_to_uint16 u
@@ -109,6 +125,7 @@ let cast #t #l t' l' u  =
   | U8, S16 -> FStar.Int.Cast.uint8_to_int16 u
   | U8, S32 -> FStar.Int.Cast.uint8_to_int32 u
   | U8, S64 -> FStar.Int.Cast.uint8_to_int64 u
+  | U8, S128 -> pow2_le_compat ((bits t')-1) (bits t); mk_int #S128 #l' (uint_v u)
   | U16, U1 -> FStar.Int.Cast.uint16_to_uint8 (FStar.UInt16.rem u 2us)
   | U16, U8 -> FStar.Int.Cast.uint16_to_uint8 u
   | U16, U16 -> u
@@ -119,6 +136,7 @@ let cast #t #l t' l' u  =
   | U16, S16 -> FStar.Int.Cast.uint16_to_int16 u
   | U16, S32 -> FStar.Int.Cast.uint16_to_int32 u
   | U16, S64 -> FStar.Int.Cast.uint16_to_int64 u
+  | U16, S128 -> pow2_le_compat ((bits t')-1) (bits t); mk_int #S128 #l' (uint_v u)
   | U32, U1 -> FStar.Int.Cast.uint32_to_uint8 (FStar.UInt32.rem u 2ul)
   | U32, U8 -> FStar.Int.Cast.uint32_to_uint8 u
   | U32, U16 -> FStar.Int.Cast.uint32_to_uint16 u
@@ -129,6 +147,7 @@ let cast #t #l t' l' u  =
   | U32, S16 -> FStar.Int.Cast.uint32_to_int16 u
   | U32, S32 -> FStar.Int.Cast.uint32_to_int32 u
   | U32, S64 -> FStar.Int.Cast.uint32_to_int64 u
+  | U32, S128 -> pow2_le_compat ((bits t')-1) (bits t); mk_int #S128 #l' (uint_v u)
   | U64, U1 -> FStar.Int.Cast.uint64_to_uint8 (FStar.UInt64.rem u 2uL)
   | U64, U8 -> FStar.Int.Cast.uint64_to_uint8 u
   | U64, U16 -> FStar.Int.Cast.uint64_to_uint16 u
@@ -139,6 +158,7 @@ let cast #t #l t' l' u  =
   | U64, S16 -> FStar.Int.Cast.uint64_to_int16 u
   | U64, S32 -> FStar.Int.Cast.uint64_to_int32 u
   | U64, S64 -> FStar.Int.Cast.uint64_to_int64 u
+  | U64, S128 -> pow2_le_compat ((bits t')-1) (bits t); mk_int #S128 #l' (uint_v u)
   | U128, U1 ->
     assert_norm (pow2 64 * pow2 64 = pow2 128);
     assert_norm (pow2 8 * pow2 56 = pow2 64);
@@ -191,42 +211,53 @@ let cast #t #l t' l' u  =
     assert_norm (pow2 64 * pow2 64 = pow2 128);
     FStar.Math.Lemmas.modulo_modulo_lemma (uint_v u) (pow2 64) (pow2 64);
     FStar.Int.Cast.uint64_to_int64 (FStar.UInt128.uint128_to_uint64 u)  
+  | U128, S128 -> mk_int #S128 #l' (uint_v u @%. t')
   | S8, U1 -> FStar.UInt8.rem (FStar.Int.Cast.int8_to_uint8 u) 2uy
   | S8, U8 -> FStar.Int.Cast.int8_to_uint8 u
   | S8, U16 -> FStar.Int.Cast.int8_to_uint16 u
   | S8, U32 -> FStar.Int.Cast.int8_to_uint32 u
   | S8, U64 -> FStar.Int.Cast.int8_to_uint64 u
+  | S8, U128 -> pow2_le_compat (bits t') ((bits t)-1); mk_int #U128 #l' (sint_v u % modulus U128)
   | S8, S8 -> u
   | S8, S16 -> FStar.Int.Cast.int8_to_int16 u
   | S8, S32 -> FStar.Int.Cast.int8_to_int32 u
   | S8, S64 -> FStar.Int.Cast.int8_to_int64 u
+  | S8, S128 ->  pow2_le_compat ((bits t')-1) ((bits t)-1); mk_int #S128 #l' (sint_v u)
   | S16, U1 -> FStar.UInt8.rem (FStar.Int.Cast.int16_to_uint8 u) 2uy
   | S16, U8 -> FStar.Int.Cast.int16_to_uint8 u
   | S16, U16 -> FStar.Int.Cast.int16_to_uint16 u
   | S16, U32 -> FStar.Int.Cast.int16_to_uint32 u
   | S16, U64 -> FStar.Int.Cast.int16_to_uint64 u
+  | S16, U128 -> pow2_le_compat (bits t') ((bits t)-1); mk_int #U128 #l' (sint_v u % modulus U128)
   | S16, S8 -> FStar.Int.Cast.int16_to_int8 u
   | S16, S16 -> u
   | S16, S32 -> FStar.Int.Cast.int16_to_int32 u
   | S16, S64 -> FStar.Int.Cast.int16_to_int64 u
+  | S16, S128 -> pow2_le_compat ((bits t')-1) ((bits t)-1); mk_int #S128 #l' (sint_v u)
   | S32, U1 -> FStar.UInt8.rem (FStar.Int.Cast.int32_to_uint8 u) 2uy
   | S32, U8 -> FStar.Int.Cast.int32_to_uint8 u
   | S32, U16 -> FStar.Int.Cast.int32_to_uint16 u
   | S32, U32 -> FStar.Int.Cast.int32_to_uint32 u
   | S32, U64 -> FStar.Int.Cast.int32_to_uint64 u
+  | S32, U128 -> pow2_le_compat (bits t') ((bits t)-1); mk_int #U128 #l' (sint_v u % modulus U128)
   | S32, S8 -> FStar.Int.Cast.int32_to_int8 u
   | S32, S16 -> FStar.Int.Cast.int32_to_int16 u
   | S32, S32 -> u
   | S32, S64 -> FStar.Int.Cast.int32_to_int64 u
+  | S32, S128 -> pow2_le_compat ((bits t')-1) ((bits t)-1); mk_int #S128 #l' (sint_v u)
   | S64, U1 -> FStar.UInt8.rem (FStar.Int.Cast.int64_to_uint8 u) 2uy
   | S64, U8 -> FStar.Int.Cast.int64_to_uint8 u
   | S64, U16 -> FStar.Int.Cast.int64_to_uint16 u
   | S64, U32 -> FStar.Int.Cast.int64_to_uint32 u
   | S64, U64 -> FStar.Int.Cast.int64_to_uint64 u
+  | S64, U128 -> pow2_le_compat (bits t') ((bits t)-1); mk_int #U128 #l' (sint_v u % modulus U128)
   | S64, S8 -> FStar.Int.Cast.int64_to_int8 u
   | S64, S16 -> FStar.Int.Cast.int64_to_int16 u
   | S64, S32 -> FStar.Int.Cast.int64_to_int32 u
   | S64, S64 -> u
+  | S64, S128 -> pow2_le_compat ((bits t')-1) ((bits t)-1); mk_int #S128 #l' (sint_v u)
+  | S128, S128 -> u
+  | S128, _ -> mk_int #t' #l' (sint_v u @%. t')
   
 
 let add_mod #t #l a b =
@@ -241,7 +272,7 @@ let add_mod #t #l a b =
   | S16 -> Int16.int_to_t (Int.add_mod (Int16.v a) (Int16.v b))
   | S32 -> Int32.int_to_t (Int.add_mod (Int32.v a) (Int32.v b))
   | S64 -> Int64.int_to_t (Int.add_mod (Int64.v a) (Int64.v b))
-  
+  | S128 -> Int128.int_to_t (Int.add_mod (Int128.v a) (Int128.v b))
 
 let add_mod_lemma #t #l a b = ()
 
@@ -257,6 +288,7 @@ let add #t #l a b =
   | S16 -> Int16.add a b
   | S32 -> Int32.add a b
   | S64 -> Int64.add a b
+  | S128 -> Int128.add a b
   
 let add_lemma #t #l a b = ()
 
@@ -272,6 +304,7 @@ let incr #t #l a =
   | S16 -> Int16.add a 0x1s
   | S32 -> Int32.add a 0x1l
   | S64 -> Int64.add a 0x1L
+  | S128 -> Int128.add a (Int128.int_to_t 1)
   
 let incr_lemma #t #l a = ()
 
@@ -307,6 +340,10 @@ let mul64_wide a b = UInt128.mul_wide a b
 
 let mul64_wide_lemma a b = ()
 
+let mul_s64_wide a b = Int128.mul_wide a b
+
+let mul_s64_wide_lemma a b = ()
+
 let sub_mod #t #l a b =
   match t with
   | U1   -> UInt8.rem (UInt8.sub_mod a b) 0x2uy
@@ -319,6 +356,7 @@ let sub_mod #t #l a b =
   | S16 -> Int16.int_to_t (Int.sub_mod (Int16.v a) (Int16.v b))
   | S32 -> Int32.int_to_t (Int.sub_mod (Int32.v a) (Int32.v b))
   | S64 -> Int64.int_to_t (Int.sub_mod (Int64.v a) (Int64.v b))
+  | S128 -> Int128.int_to_t (Int.sub_mod (Int128.v a) (Int128.v b))
 
 let sub_mod_lemma #t #l a b = ()
 
@@ -334,7 +372,8 @@ let sub #t #l a b =
   | S16 -> Int16.sub a b
   | S32 -> Int32.sub a b
   | S64 -> Int64.sub a b
-
+  | S128 -> Int128.sub a b
+  
 let sub_lemma #t #l a b = ()
 
 let decr #t #l a =
@@ -349,10 +388,12 @@ let decr #t #l a =
   | S16 -> Int16.sub a 0x1s
   | S32 -> Int32.sub a 0x1l
   | S64 -> Int64.sub a 0x1L
-  
-let decr_lemma #t #l a = ()
+  | S128 -> Int128.sub a (Int128.int_to_t 1)
 
+let decr_lemma #t #l a = ()
+ 
 #reset-options "--z3rlimit 300"
+
 let logxor #t #l a b =
   match t with
   | U1   ->
@@ -370,50 +411,51 @@ let logxor #t #l a b =
   | S16 -> Int16.logxor a b
   | S32 -> Int32.logxor a b
   | S64 -> Int64.logxor a b
+  | S128 -> Int128.logxor a b
   
-#set-options "--max_fuel 1"
+#set-options "--max_fuel 1" 
 
-val logxor_lemma_: #t:inttype -> a:uint_t t SEC -> b:uint_t t SEC -> Lemma
-  (uint_v (a `logxor` (a `logxor` b)) == uint_v b)
-let logxor_lemma_ #t a b =
+val logxor_lemma_: #t:inttype -> #l:secrecy_level -> a:int_t t l -> b:int_t t l -> Lemma
+  (int_v (a `logxor` (a `logxor` b)) == int_v b)
+let logxor_lemma_ #t #l a b =
   match t with
   |U1 |U8 |U16 |U32 |U64 |U128 ->
   UInt.logxor_associative #(bits t) (uint_v a) (uint_v a) (uint_v b);
   UInt.logxor_self #(bits t) (uint_v a);
   UInt.logxor_commutative #(bits t) 0 (uint_v b);
   UInt.logxor_lemma_1 #(bits t) (uint_v b)
-  |S8 |S16 |S32 |S64 ->
-  Int.logxor_associative #(bits t) (uint_v a) (uint_v a) (uint_v b);
-  Int.logxor_self #(bits t) (uint_v a);
-  Int.logxor_commutative #(bits t) 0 (uint_v b);
-  Int.logxor_lemma_1 #(bits t) (uint_v b)
+  |S8 |S16 |S32 |S64 |S128 ->
+  Int.logxor_associative #(bits t) (sint_v a) (sint_v a) (sint_v b);
+  Int.logxor_self #(bits t) (sint_v a);
+  Int.logxor_commutative #(bits t) 0 (sint_v b);
+  Int.logxor_lemma_1 #(bits t) (sint_v b)
 
-let logxor_lemma #t a b =
+let logxor_lemma #t #l a b =
   logxor_lemma_ #t a b;
-  uintv_extensionality (logxor a (logxor a b)) b;
+  intv_extensionality (logxor a (logxor a b)) b;
   assert (a `logxor` (a `logxor` b) == b);
   (match t with |U1 |U8 |U16 |U32 |U64 |U128 ->
    UInt.logxor_commutative #(bits t) (uint_v a) (uint_v b)
-   |S8 |S16 |S32 |S64 -> Int.logxor_commutative #(bits t) (uint_v a) (uint_v b));
+   |S8 |S16 |S32 |S64 |S128 -> Int.logxor_commutative #(bits t) (sint_v a) (sint_v b));
   logxor_lemma_ #t a b;
-  uintv_extensionality (logxor a (logxor b a)) b;
+  intv_extensionality (logxor a (logxor b a)) b;
   assert ((a `logxor` (b `logxor` a)) == b);
   (match t with |U1 |U8 |U16 |U32 |U64 |U128 ->
    UInt.logxor_lemma_1 #(bits t) (uint_v a)
-   |S8 |S16 |S32 |S64 -> Int.logxor_lemma_1 #(bits t) (uint_v a));
+   |S8 |S16 |S32 |S64 |S128 -> Int.logxor_lemma_1 #(bits t) (sint_v a));
   //UInt.logxor_lemma_1 #(bits t) (uint_v a);
-  uintv_extensionality (logxor a (uint #t #SEC 0)) a
+  intv_extensionality (logxor a (mk_int #t #l 0)) a
 
-let logxor_lemma1 #t a b =
+let logxor_lemma1 #t #l a b =
   match (v a, v b) with
   | _, 0 ->
-    UInt.logxor_lemma_1 #(bits t) (uint_v a)
+    UInt.logxor_lemma_1 #(bits t) (int_v a)
   | 0, _ ->
-    UInt.logxor_commutative #(bits t) (uint_v a) (uint_v b);
-    UInt.logxor_lemma_1 #(bits t) (uint_v b)
+    UInt.logxor_commutative #(bits t) (int_v a) (int_v b);
+    UInt.logxor_lemma_1 #(bits t) (int_v b)
   | 1, 1 ->
-    uintv_extensionality a b;
-    UInt.logxor_self #(bits t) (uint_v a)
+    intv_extensionality a b;
+    UInt.logxor_self #(bits t) (int_v a)
 
 #set-options "--max_fuel 0"
 
@@ -434,23 +476,26 @@ let logand #t #l a b =
   | S16 -> Int16.logand a b
   | S32 -> Int32.logand a b
   | S64 -> Int64.logand a b
-
+  | S128 -> Int128.logand a b
 
 let logand_lemma #t a b =
-  match t with |U1 |U8 |U16 |U32 |U64 |U128 ->
+  match t with 
+  |U8 |U16 |U32 |U64 |U128 ->
    if (uint_v a = 0) then begin
     UInt.logand_commutative #(bits t) (uint_v a) (uint_v b);
     UInt.logand_lemma_1 #(bits t) (uint_v b) end
   else begin
     UInt.logand_commutative #(bits t) (uint_v a) (uint_v b);
     UInt.logand_lemma_2 #(bits t) (uint_v b) end
-  |S8 |S16 |S32 |S64 ->
-   if (uint_v a = 0) then begin
-    Int.logand_commutative #(bits t) (uint_v a) (uint_v b);
-    Int.logand_lemma_1 #(bits t) (uint_v b) end
+  |S8 |S16 |S32 |S64 | S128 ->
+   if (sint_v a = 0) then begin
+    Int.logand_commutative #(bits t) (sint_v a) (sint_v b);
+    Int.logand_lemma_1 #(bits t) (sint_v b) end
   else begin
-    Int.logand_commutative #(bits t) (uint_v a) (uint_v b);
-    Int.logand_lemma_2 #(bits t) (uint_v b) end
+    Int.logand_commutative #(bits t) (sint_v a) (sint_v b);
+    Int.logand_lemma_2 #(bits t) (sint_v b) end
+
+#reset-options "--z3rlimit 300"
 
 let logand_spec #t #l a b = ()
 
@@ -471,7 +516,8 @@ let logor #t #l a b =
   | S16 -> Int16.logor a b
   | S32 -> Int32.logor a b
   | S64 -> Int64.logor a b
-
+  | S128 -> Int128.logor a b
+  
 let logor_spec #t #l a b = ()
 
 #set-options "--max_fuel 1"
@@ -499,7 +545,8 @@ let lognot #t #l a =
   | S16 -> Int16.lognot a
   | S32 -> Int32.lognot a
   | S64 -> Int64.lognot a
-
+  | S128 -> Int128.lognot a
+  
 let shift_right_negative (#n:pos) (a:Int.int_t n{a < 0}) (s:nat) : Tot (Int.int_t n) =
   let shift_right_negative_vec (#n:pos) (a:BitVector.bv_t n) (s:nat) : Tot (BitVector.bv_t n) =
   if s>= n then BitVector.ones_vec #n
@@ -519,7 +566,7 @@ let shift_right #t #l a b =
   | S16 -> Int16.shift_arithmetic_right a b
   | S32 -> Int32.shift_arithmetic_right a b
   | S64 -> Int64.shift_arithmetic_right a b
-
+  | S128 -> Int128.shift_arithmetic_right a b
 
 #reset-options "--z3rlimit 500 --max_fuel 2 --max_ifuel 2"
 
@@ -545,15 +592,15 @@ let shift_right_value_aux_2 #n a = assert_norm (pow2 0 == 1)
 
 #reset-options "--z3rlimit 500 --max_fuel 2 --max_ifuel 2"
 
-val append_lemma: #n:pos -> #m:pos -> a:BitVector.bv_t n -> b:BitVector.bv_t m ->
-  Lemma (Int.from_vec #(n + m) (Seq.append a b) = (Int.from_vec #n a) * pow2 m + (UInt.from_vec #m b))
-let append_lemma #n #m a b =
-  let a1 = Int.from_vec #n a in
-  let a2 = UInt.from_vec #n a in
-  let b' = UInt.from_vec #m b in
-  let s1 = Int.from_vec #(n+m) (Seq.append a b) in
-  let s2 = UInt.from_vec #(n+m) (Seq.append a b) in
-  admit()
+// val append_lemma: #n:pos -> #m:pos -> a:BitVector.bv_t n -> b:BitVector.bv_t m ->
+//   Lemma (Int.from_vec #(n + m) (Seq.append a b) = (Int.from_vec #n a) * pow2 m + (UInt.from_vec #m b))
+// let append_lemma #n #m a b =
+//   let a1 = Int.from_vec #n a in
+//   let a2 = UInt.from_vec #n a in
+//   let b' = UInt.from_vec #m b in
+//   let s1 = Int.from_vec #(n+m) (Seq.append a b) in
+//   let s2 = UInt.from_vec #(n+m) (Seq.append a b) in
+//   admit()
 
 val shift_right_value_aux_0: #n:pos{n > 1} -> a:Int.int_t n ->
   Lemma (requires True)
@@ -611,9 +658,9 @@ let rec shift_right_value_aux_3 #n a s =
 let shift_right_lemma #t #l a b = 
   match t with
   |U1 |U8 |U16 |U32 |U64 |U128 -> ()
-  |_ -> if (uint_v b >= bits t) then shift_right_value_aux_1 #(bits t) (uint_v a) (uint_v b)
-       else if (uint_v b = 0) then shift_right_value_aux_2 #(bits t) (uint_v a)
-       else shift_right_value_aux_3 #(bits t) (uint_v a) (uint_v b)
+  |S8 |S16 |S32 |S64 |S128 -> if (int_v b >= bits t) then shift_right_value_aux_1 #(bits t) (int_v a) (int_v b)
+       else if (int_v b = 0) then shift_right_value_aux_2 #(bits t) (int_v a)
+       else shift_right_value_aux_3 #(bits t) (int_v a) (int_v b)
   
 let shift_left_negative (#n:pos) (a:Int.int_t n{a < 0}) (s:nat) : Tot (Int.int_t n) =
   FStar.Int.from_vec (BitVector.shift_left_vec #n (FStar.Int.to_vec #n a) s)
@@ -626,22 +673,24 @@ let shift_left #t #l a b =
   | U32  -> UInt32.shift_left a b
   | U64  -> UInt64.shift_left a b
   | U128 -> UInt128.shift_left a b
-  | S8 -> if (uint_v a >= 0) then Int8.shift_left a b
+  | S8 -> if (sint_v a >= 0) then Int8.shift_left a b
          else Int8.int_to_t (shift_left_negative (Int8.v a) (UInt32.v b))
-  | S16 -> if (uint_v a >= 0) then Int16.shift_left a b
+  | S16 -> if (sint_v a >= 0) then Int16.shift_left a b
          else Int16.int_to_t (shift_left_negative (Int16.v a) (UInt32.v b))
-  | S32 -> if (uint_v a >= 0) then Int32.shift_left a b
+  | S32 -> if (sint_v a >= 0) then Int32.shift_left a b
          else Int32.int_to_t (shift_left_negative (Int32.v a) (UInt32.v b))
-  | S64 -> if (uint_v a >= 0) then Int64.shift_left a b
+  | S64 -> if (sint_v a >= 0) then Int64.shift_left a b
          else Int64.int_to_t (shift_left_negative (Int64.v a) (UInt32.v b))
-
+  | S128 -> if (sint_v a >= 0) then Int128.shift_left a b
+         else Int128.int_to_t (shift_left_negative (Int128.v a) (UInt32.v b))
+         
 #reset-options "--z3rlimit 800 --max_fuel 3 --max_ifuel 3"
 
 let shift_left_lemma #t #l a b = 
   match t with
   |U1 |U8 |U16 |U32 |U64 |U128 -> ()
-  |_ -> let a' = uint_v a in
-       let b' = uint_v b in
+  |_ -> let a' = int_v a in
+       let b' = int_v b in
        let n = Int.to_uint a' in
        let sn = UInt.shift_left #(bits t) n b' in
        assert(Int.to_vec a' == UInt.to_vec #(bits t) n); 
@@ -666,7 +715,7 @@ let rotate_right #t #l a b =
 let rotate_left #t #l a b =
   logor (shift_left a b) (shift_right a (sub #U32 (size (bits t)) b))
 
-let zeroes t l = nat_to_uint #t #l 0
+let zeroes t l = nat_to_int #t #l 0
 
 let ones t l =
   match t with
@@ -680,11 +729,11 @@ let ones t l =
     let y = (UInt128.shift_left x 64ul) `UInt128.add` x in
     assert_norm (UInt128.v y == pow2 128 - 1);
     y
-  | _  -> uint #t #l (ones_v t)
+  | _  -> mk_int #t #l (ones_v t)
 
 inline_for_extraction
-let minus (#t:inttype) (#l:secrecy_level) (a:uint_t t l) = add_mod (lognot a) (uint #t #l 1)
- 
+let minus (#t:inttype) (#l:secrecy_level) (a:int_t t l) = add_mod (lognot a) (mk_int #t #l 1)
+
 let eq_mask #t a b =
   match t with
   | U1   -> lognot (logxor a b)
@@ -697,6 +746,7 @@ let eq_mask #t a b =
   | S16  -> to_i16 (UInt16.eq_mask (to_u16 a) (to_u16 b))
   | S32  -> to_i32 (UInt32.eq_mask (to_u32 a) (to_u32 b))
   | S64  -> to_i64 (UInt64.eq_mask (to_u64 a) (to_u64 b))
+  | S128 -> to_i128 (UInt128.eq_mask (to_u128 a) (to_u128 b))
 
 #reset-options "--z3rlimit 3000 --max_fuel 1 --max_ifuel 1"
 
@@ -757,6 +807,20 @@ let eq_mask_lemma #t a b =
       assert(v a' <> v b');
       assert(v m' = 0);
       assert(v (to_i64 m') = 0) end
+  | S128 -> let a' = to_u128 a in let b' = to_u128 b in
+    assert (v a = v a' @% pow2 128); assert( v a' = v a % pow2 128);
+    assert (v b = v b' @% pow2 128); assert( v b' = v b % pow2 128);
+    let m' = UInt64.eq_mask a' b' in
+    assert (v a' = v b' ==> v m' = ones_v U64);
+    assert (v a' <> v b' ==> v m' = 0);
+    if (v a = v b) then begin
+      assert (v a' = v b');
+      assert (v m' = ones_v U64);
+      assert (v (to_i128 m') = -1) end
+    else begin
+      assert(v a' <> v b');
+      assert(v m' = 0);
+      assert(v (to_i128 m') = 0) end
 
 let eq_mask_logand_lemma #t a b c =
   eq_mask_lemma a b;
@@ -799,32 +863,45 @@ let gt_mask #t a b = logand (gte_mask a b) (neq_mask a b)
 let lte_mask #t a b = logor (lt_mask a b) (eq_mask a b)
 
 #reset-options "--z3rlimit 3000 --max_fuel 3 --max_ifuel 3"
+
 private
-val mod_mask_value: #t:inttype{~(S8? t) /\ ~(S16? t) /\ ~(S32? t) /\ ~(S64? t)} -> #l:secrecy_level -> m:shiftval t ->
-  Lemma (uint_v (mod_mask #t #l m) == pow2 (uint_v m) - 1)
+val mod_mask_value: #t:inttype -> #l:secrecy_level -> m:shiftval t ->
+  Lemma (int_v (mod_mask #t #l m) == pow2 (uint_v m) - 1)
+
 let mod_mask_value #t #l m =
-  if uint_v m > 0 then begin
-    let m = uint_v m in
-    pow2_lt_compat (bits t) m;
-    small_modulo_lemma_1 (pow2 m) (pow2 (bits t));
-    assert (FStar.Mul.(1 * pow2 m) == pow2 m);
-    UInt.shift_left_value_lemma #(bits t) 1 m
-  end
+  shift_left_lemma (nat_to_int #t #l 1) m;
+  pow2_double_mult ((bits t) - 1);
+  pow2_le_compat (uint_v m) 0;
+  pow2_lt_compat (bits t) (uint_v m);
+  small_modulo_lemma_1 (pow2 (uint_v m)) (pow2 (bits t));
+  small_modulo_lemma_1 ((pow2 (uint_v m)) -1) (pow2 (bits t));
+  assert( int_v (mod_mask #t #l m) == (((1 * pow2 (uint_v m)) @%. t) - 1) @%. t);
+  match t with
+  |U1 |U8 |U16 |U32 |U64 |U128 -> ()
+  |_ -> if (uint_v m < (bits t) -1) then (pow2_lt_compat ((bits t)-1) (uint_v m); assert((1*pow2 (uint_v m))@%. t = pow2 (uint_v m))) else (assert ((1* pow2 (uint_v m)) @%. t = pow2 (uint_v m) - pow2 (bits t)); assert (uint_v m = (bits t) -1); pow2_double_mult ((bits t) -1); assert ((1 * pow2 (uint_v m)) @%. t = - pow2 (uint_v m))) 
 
 #set-options "--max_fuel 1"
 
 let mod_mask_lemma #t #l a m =
   mod_mask_value #t #l m;
+  match t with
+  |U1 |U8 |U16 |U32 |U64 |U128 ->
   if uint_v m = 0 then
     UInt.logand_lemma_1 #(bits t) (uint_v a)
   else
-    UInt.logand_mask #(bits t) (uint_v a) (uint_v m)
-
+    UInt.logand_mask #(bits t) (uint_v a) (uint_v m) 
+  |_->
+  if uint_v m = 0 then
+    Int.logand_lemma_1 #(bits t) (sint_v a)
+  else admit() 
+  
 #set-options "--max_fuel 0"
 
 (* defined in .fsti: notations +^, -^, ...*)
 
 let nat_mod_v #m x = x
+
+#reset-options "--z3rlimit 3000 --max_fuel 1 --max_ifuel 1"
 
 let div #t x y =
   match t with
@@ -833,6 +910,10 @@ let div #t x y =
   | U16 -> UInt16.div x y
   | U32 -> UInt32.div x y
   | U64 -> UInt64.div x y
+  //| S8 -> Int8.div x y
+  //| S16 -> Int16.div x y
+  //| S32 -> Int32.div x y
+  //| S64 -> Int64.div x y
   
 let div_lemma #t x y = ()
 
@@ -843,7 +924,11 @@ let mod #t x y =
   | U16 -> UInt16.rem x y
   | U32 -> UInt32.rem x y
   | U64 -> UInt64.rem x y
-
+  //| S8 -> Int8.rem x y
+  //| S16 -> Int16.rem x y
+  //| S32 -> Int32.rem x y
+  //| S64 -> Int64.rem x y
+  
 let mod_lemma #t x y = ()
 
 let eq #t x y =
@@ -858,7 +943,8 @@ let eq #t x y =
   | S16 -> Int16.eq x y
   | S32 -> Int32.eq x y
   | S64 -> Int64.eq x y
-  
+  | S128 -> Int128.eq x y
+
 let eq_lemma #t x y = ()
 
 let ne #t x y =
@@ -873,6 +959,7 @@ let ne #t x y =
   | S16 -> not (Int16.eq x y)
   | S32 -> not (Int32.eq x y)
   | S64 -> not (Int64.eq x y)
+  | S128 -> not (Int128.eq x y)
   
 let ne_lemma #t x y = ()
 
@@ -888,6 +975,7 @@ let lt #t x y =
   | S16 -> Int16.lt x y
   | S32 -> Int32.lt x y
   | S64 -> Int64.lt x y
+  | S128 -> Int128.lt x y
   
 let lt_lemma #t x y = ()
 
@@ -903,6 +991,7 @@ let lte #t x y =
   | S16 -> Int16.lte x y
   | S32 -> Int32.lte x y
   | S64 -> Int64.lte x y
+  | S128 -> Int128.lte x y
   
 let lte_lemma #t x y = ()
 
@@ -918,6 +1007,7 @@ let gt #t x y =
   | S16 -> Int16.gt x y
   | S32 -> Int32.gt x y
   | S64 -> Int64.gt x y
+  | S128 -> Int128.gt x y
   
 let gt_lemma #t x y = ()
 
@@ -933,5 +1023,6 @@ let gte #t x y =
   | S16 -> Int16.gte x y
   | S32 -> Int32.gte x y
   | S64 -> Int64.gte x y
+  | S128 -> Int128.gte x y
   
 let gte_lemma #t x y = ()
