lib/Lib.IntTypes.fsti
@@ -8,7 +8,23 @@ open FStar.Math.Lemmas
 ///
 
 type inttype =
-  | U1 | U8 | U16 | U32 | U64 | U128 | S8 | S16 | S32 | S64
+  | U1 | U8 | U16 | U32 | U64 | U128 | S8 | S16 | S32 | S64 | S128
+
+let unsigned (i:inttype) =
+  i = U1 ||
+  i = U8 ||
+  i = U16 ||
+  i = U32 ||
+  i = U64 ||
+  i = U128
+let signed (i:inttype) =
+  i = S8 ||
+  i = S16 ||
+  i = S32 ||
+  i = S64 ||
+  i = S128
+
+
 ///
 /// Operations on the underlying machine integer base types
 ///
@@ -26,7 +42,7 @@ let bits (n:inttype) =
   | U64 -> 64
   | S64 -> 64
   | U128 -> 128
-  //| S128 -> 128
+  | S128 -> 128
 
 
 val pow2_values: n:nat ->  Lemma (
@@ -48,20 +64,18 @@ unfold let modulus (t:inttype) = pow2 (bits t)
 
 inline_for_extraction
 unfold let maxint (t:inttype) =
-  match t with
-  | U1 | U8 | U16 | U32 | U64 | U128 -> pow2 (bits t) - 1
-  | S8 | S16 | S32 | S64 -> pow2 ((bits t) -1) - 1
-  
+  if (unsigned t) then pow2 (bits t) - 1
+  else (assert(signed t); (pow2 ((bits t) - 1)) - 1)
+
 inline_for_extraction
 unfold let minint (t:inttype) =
-  match t with
-  | U1 | U8 | U16 | U32 | U64 | U128 -> 0
-  | S8 | S16 | S32 | S64 -> - (pow2 ((bits t)-1))
+  if (unsigned t) then 0
+  else - (pow2 ((bits t) - 1))
 
 inline_for_extraction
 let range (x:int) (n:inttype) : Type0 =
   minint n <= x /\ x <= maxint n
-  
+
 inline_for_extraction
 type range_t (n:inttype) = x:int{range x n}
 
@@ -78,9 +92,9 @@ let numbytes (n:inttype) =
   | U64 -> 8
   | S64 -> 8
   | U128 -> 16
-  //| S128 -> 16
+  | S128 -> 16
 
-  
+
 (* PUBLIC Machine Integers *)
 
 inline_for_extraction
@@ -96,7 +110,7 @@ let pub_int_t (t:inttype) =
   | S16 -> Int16.t
   | S32 -> Int32.t
   | S64 -> Int64.t
-  //| S128 -> Int128.t
+  | S128 -> Int128.t
 
 inline_for_extraction
 let pub_int_v #t (x:pub_int_t t) : (n:range_t t) =
@@ -111,7 +125,7 @@ let pub_int_v #t (x:pub_int_t t) : (n:range_t t) =
   | S16 -> Int16.v x
   | S32 -> Int32.v x
   | S64 -> Int64.v x
-  //| S128 -> Int128.v x
+  | S128 -> Int128.v x
 
 (* SECRET Machine Integers *)
 
@@ -128,24 +142,25 @@ val sec_int_v: #t:inttype -> u:sec_int_t t -> n:range_t t
 (* GENERIC (unsigned) Machine Integers *)
 
 inline_for_extraction
-let uint_t (t:inttype) (l:secrecy_level) =
+let int_t (t:inttype) (l:secrecy_level) =
   match l with
   | PUB -> pub_int_t t
   | SEC -> sec_int_t t
 
-let uint_v #t #l (u:uint_t t l) : n:range_t t =
+let int_v #t #l (u:int_t t l) : n:range_t t =
   match l with
   | PUB -> pub_int_v #t u
   | SEC -> sec_int_v #t u
 
-val uintv_extensionality:
-   #t:inttype
- -> #l:secrecy_level
- -> a:uint_t t l
- -> b:uint_t t l
- -> Lemma
-  (requires uint_v #t #l a == uint_v #t #l b)
-  (ensures  a == b)
+inline_for_extraction
+let uint_t (t:inttype{unsigned t}) (l:secrecy_level) = int_t t l
+
+inline_for_extraction
+let sint_t (t:inttype{signed t}) (l:secrecy_level) = int_t t l
+
+
+let uint_v #t #l (u:uint_t t l) = int_v u
+let sint_v #t #l (u:sint_t t l) = int_v u
 
 ///
 /// Definition of machine integers
@@ -158,31 +173,31 @@ inline_for_extraction
 type uint8 = uint_t U8 SEC
 
 inline_for_extraction
-type int8 = uint_t S8 SEC
+type int8 = sint_t S8 SEC
 
 inline_for_extraction
 type uint16 = uint_t U16 SEC
 
 inline_for_extraction
-type int16 = uint_t S16 SEC
+type int16 = sint_t S16 SEC
 
 inline_for_extraction
 type uint32 = uint_t U32 SEC
 
 inline_for_extraction
-type int32 = uint_t S32 SEC
+type int32 = sint_t S32 SEC
 
 inline_for_extraction
 type uint64 = uint_t U64 SEC
 
 inline_for_extraction
-type int64 = uint_t S64 SEC
+type int64 = sint_t S64 SEC
 
 inline_for_extraction
 type uint128 = uint_t U128 SEC
 
-//inline_for_extraction
-//type int128 = uint_t S128 SEC
+inline_for_extraction
+type int128 = sint_t S128 SEC
 
 inline_for_extraction
 unfold type bit_t = uint_t U1 PUB
@@ -194,47 +209,53 @@ inline_for_extraction
 unfold type size_t = uint_t U32 PUB
 
 inline_for_extraction
-unfold type pub_int8 = uint_t S8 PUB
+unfold type pub_int8 = sint_t S8 PUB
 
 inline_for_extraction
 unfold type pub_uint16 = uint_t U16 PUB
 
 inline_for_extraction
-unfold type pub_int16 = uint_t S16 PUB
+unfold type pub_int16 = sint_t S16 PUB
 
 inline_for_extraction
 unfold type pub_uint32 = uint_t U32 PUB
 
 inline_for_extraction
-unfold type pub_int32 = uint_t S32 PUB
+unfold type pub_int32 = sint_t S32 PUB
 
 inline_for_extraction
 unfold type pub_uint64 = uint_t U64 PUB
 
 inline_for_extraction
-unfold type pub_int64 = uint_t S64 PUB
+unfold type pub_int64 = sint_t S64 PUB
 
 inline_for_extraction
 unfold type pub_uint128 = uint_t U128 PUB
 
-//inline_for_extraction
-//unfold type pub_int128 = uint_t S128 PUB
+inline_for_extraction
+unfold type pub_int128 = sint_t S128 PUB
 ///
 /// Casts between natural numbers and machine integers
 ///
 
 inline_for_extraction
-val secret: #t:inttype -> u:uint_t t PUB -> v:uint_t t SEC{uint_v v == uint_v u}
+val secret: #t:inttype -> u:int_t t PUB -> v:int_t t SEC{int_v v == int_v u}
 
 inline_for_extraction
-val uint: #t:inttype -> #l:secrecy_level -> (n:range_t t) -> u:uint_t t l{uint_v u == n}
+val mk_int: #t:inttype -> #l:secrecy_level -> (n:range_t t) -> u:int_t t l{int_v u == n}
 
-val uintv_injective:
+inline_for_extraction
+let uint (#t:inttype{unsigned t}) (#l:secrecy_level) (n:range_t t) = mk_int #t #l n
+
+inline_for_extraction
+let sint (#t:inttype{signed t}) (#l:secrecy_level) (n:range_t t) = mk_int #t #l n
+
+val intv_injective:
    #t:inttype
  -> #l:secrecy_level
- -> a:uint_t t l
- -> Lemma (ensures uint (uint_v #t #l a) == a)
- [SMTPat (uint_v #t #l a)]
+ -> a:int_t t l
+ -> Lemma (ensures mk_int (int_v #t #l a) == a)
+ [SMTPat (int_v #t #l a)]
 
 inline_for_extraction
 let u1 (n:range_t U1) : u:uint1{uint_v #U1 u == n} = uint #U1 #SEC n
@@ -243,32 +264,35 @@ inline_for_extraction
 let u8 (n:range_t U8) : u:uint8{uint_v #U8 u == n} = uint #U8 #SEC n
 
 inline_for_extraction
-let i8 (n:range_t S8) : u:int8{uint_v #S8 u == n} = uint #S8 #SEC n
+let i8 (n:range_t S8) : u:int8{sint_v #S8 u == n} = sint #S8 #SEC n
 
 inline_for_extraction
 let u16 (n:range_t U16) : u:uint16{uint_v #U16 u == n} = uint #U16 #SEC n
 
 inline_for_extraction
-let i16 (n:range_t S16) : u:int16{uint_v #S16 u == n} = uint #S16 #SEC n
+let i16 (n:range_t S16) : u:int16{sint_v #S16 u == n} = sint #S16 #SEC n
 
 inline_for_extraction
 let u32 (n:range_t U32) : u:uint32{uint_v #U32 u == n} = uint #U32 #SEC n
 
 inline_for_extraction
-let i32 (n:range_t S32) : u:int32{uint_v #S32 u == n} = uint #S32 #SEC n
+let i32 (n:range_t S32) : u:int32{sint_v #S32 u == n} = sint #S32 #SEC n
 
 inline_for_extraction
 let u64 (n:range_t U64) : u:uint64{uint_v #U64 u == n} = uint #U64 #SEC n
 
 inline_for_extraction
-let i64 (n:range_t S64) : u:int64{uint_v #S64 u == n} = uint #S64 #SEC n
+let i64 (n:range_t S64) : u:int64{sint_v #S64 u == n} = sint #S64 #SEC n
 
-(* We only support 64-bit literals, hence the unexpected upper limit in the following function *)
+#reset-options
+(* We only support 64-bit literals, hence the unexpected upper limit in the following functions *)
 inline_for_extraction
-val u128: (n:range_t U64) -> u:uint128{uint_v #U128 u == n}
+let u128 (n:range_t U64) : u:uint128{uint_v #U128 u == n} = uint #U128 #SEC n
 
-//inline_for_extraction
-//let i128 (n:range_t S128) : u:int128{uint_v #S128 u == n} = uint #S128 #SEC n
+inline_for_extraction
+let i128 (n:range_t S64) : u:int128{sint_v #S128 u == n} = 
+  pow2_le_compat ((bits S128) -1) ((bits S64)-1);
+  sint #S128 #SEC n
 
 unfold noextract
 let max_size_t = maxint U32
@@ -286,7 +310,7 @@ unfold inline_for_extraction
 let size_v (s:size_t) = uint_v #U32 #PUB s
 
 unfold inline_for_extraction noextract
-let v #t #l x = uint_v #t #l x
+let v #t #l x = int_v #t #l x
 
 val size_v_size_lemma: s:size_nat ->
   Lemma
@@ -320,18 +344,20 @@ inline_for_extraction
 val byte_to_int8: s:byte_t -> u:int8{u == i8 ((byte_v s) @% 256)}
 
 inline_for_extraction
-val nat_to_uint: #t:inttype -> #l:secrecy_level -> (n:range_t t) -> u:uint_t t l{uint_v u == n}
+val nat_to_int: #t:inttype -> #l:secrecy_level -> (n:range_t t) -> u:int_t t l{int_v u == n}
+
+inline_for_extraction
+let nat_to_uint (#t:inttype{unsigned t}) (#l:secrecy_level) (n:range_t t) = nat_to_int #t #l n
 
 inline_for_extraction
 let op_At_Percent_Dot x t =
-  match t with
-  | U1 | U8 | U16 | U32 | U64 | U128 -> x % modulus t
-  | S8 | S16 | S32 | S64 -> x @% modulus t
+  if (unsigned t) then x % modulus t
+  else x @% modulus t
 
 inline_for_extraction
 val cast: #t:inttype -> #l:secrecy_level
-          -> t':inttype{(~(U128? t')) \/ (U1? t) \/ (U8? t) \/ (U16? t) \/ (U32? t) \/ (U64? t) \/ (U128? t)} -> l':secrecy_level {PUB? l \/ SEC? l'}
-          -> u1:uint_t t l -> u2:uint_t t' l'{uint_v u2 == uint_v u1 @%. t'}
+          -> t':inttype -> l':secrecy_level {PUB? l \/ SEC? l'}
+          -> u1:int_t t l -> u2:int_t t' l'{int_v u2 == int_v u1 @%. t'}
 
 inline_for_extraction
 let to_u1 #t #l u : uint1 = cast #t #l U1 SEC u
@@ -361,10 +387,10 @@ inline_for_extraction
 let to_i64 #t #l u : int64 = cast #t #l S64 SEC u
 
 inline_for_extraction
-let to_u128 (#t:inttype{(U1? t) \/ (U8? t) \/ (U16? t) \/ (U32? t) \/ (U64? t) \/ (U128? t)}) #l u : uint128 = cast #t #l U128 SEC u
+let to_u128 #t #l u : uint128 = cast #t #l U128 SEC u
 
-//inline_for_extraction
-//let to_i128 #t #l u : int128 = cast #t #l S128 SEC u
+inline_for_extraction
+let to_i128 #t #l u : int128 = cast #t #l S128 SEC u
 
 ///
 /// Bitwise operators for all machine integers
@@ -372,71 +398,71 @@ let to_u128 (#t:inttype{(U1? t) \/ (U8? t) \/ (U16? t) \/ (U32? t) \/ (U64? t) \
 
 inline_for_extraction
 val add_mod: #t:inttype -> #l:secrecy_level ->
-             a:uint_t t l ->
-             b:uint_t t l ->
-             c:uint_t t l
+             a:int_t t l ->
+             b:int_t t l ->
+             c:int_t t l
 
 inline_for_extraction
 val add_mod_lemma: #t:inttype -> #l:secrecy_level ->
-             a:uint_t t l ->
-             b:uint_t t l ->
+             a:int_t t l ->
+             b:int_t t l ->
 	     Lemma
-	     (ensures (uint_v #t #l (add_mod #t #l a b) == (uint_v a + uint_v b) @%. t))
-	     [SMTPat (uint_v #t #l (add_mod #t #l a b))]
+	     (ensures (int_v #t #l (add_mod #t #l a b) == (int_v a + int_v b) @%. t))
+	     [SMTPat (int_v #t #l (add_mod #t #l a b))]
 
 inline_for_extraction
 val add: #t:inttype -> #l:secrecy_level
-  -> a:uint_t t l
-  -> b:uint_t t l{range (uint_v a + uint_v b) t}
-  -> uint_t t l
+  -> a:int_t t l
+  -> b:int_t t l{range (int_v a + int_v b) t}
+  -> int_t t l
 
 inline_for_extraction
 val add_lemma: #t:inttype -> #l:secrecy_level
-  -> a:uint_t t l
-  -> b:uint_t t l{range (uint_v a + uint_v b) t}
+  -> a:int_t t l
+  -> b:int_t t l{range (int_v a + int_v b) t}
   -> Lemma
-    (ensures (uint_v #t #l (add #t #l a b) == uint_v a + uint_v b))
-    [SMTPat (uint_v #t #l (add #t #l a b))]
+    (ensures (int_v #t #l (add #t #l a b) == int_v a + int_v b))
+    [SMTPat (int_v #t #l (add #t #l a b))]
 
 inline_for_extraction
 val incr: #t:inttype -> #l:secrecy_level
-  -> a:uint_t t l{uint_v a < maxint t}
-  -> uint_t t l
+  -> a:int_t t l{int_v a < maxint t}
+  -> int_t t l
 
 inline_for_extraction
 val incr_lemma: #t:inttype -> #l:secrecy_level
-  -> a:uint_t t l{uint_v a < maxint t}
+  -> a:int_t t l{int_v a < maxint t}
   -> Lemma
-  (ensures (uint_v #t #l (incr a) == uint_v a + 1))
+  (ensures (int_v #t #l (incr a) == int_v a + 1))
 
 inline_for_extraction
-val mul_mod: #t:inttype{t <> U128} -> #l:secrecy_level
-  -> a:uint_t t l
-  -> b:uint_t t l
-  -> uint_t t l
+val mul_mod: #t:inttype{t <> U128 /\ t <> S128} -> #l:secrecy_level
+  -> a:int_t t l
+  -> b:int_t t l
+  -> int_t t l
 
 inline_for_extraction
-val mul_mod_lemma: #t:inttype{t <> U128} -> #l:secrecy_level
-  -> a:uint_t t l
-  -> b:uint_t t l
+val mul_mod_lemma: #t:inttype{t <> U128 /\ t <> S128} -> #l:secrecy_level
+  -> a:int_t t l
+  -> b:int_t t l
   -> Lemma
-  (ensures (uint_v #t #l (mul_mod #t #l a b) == (uint_v a `op_Multiply` uint_v b) @%. t))
-  [SMTPat (uint_v #t #l (mul_mod #t #l a b))]
+  (ensures (int_v #t #l (mul_mod #t #l a b) == (int_v a `op_Multiply` int_v b) @%. t))
+  [SMTPat (int_v #t #l (mul_mod #t #l a b))]
 
 inline_for_extraction
-val mul: #t:inttype{t <> U128} -> #l:secrecy_level
-  -> a:uint_t t l
-  -> b:uint_t t l{range (uint_v a `op_Multiply` uint_v b) t}
-  -> uint_t t l
+val mul: #t:inttype{t <> U128 /\ t <> S128} -> #l:secrecy_level
+  -> a:int_t t l
+  -> b:int_t t l{range (int_v a `op_Multiply` int_v b) t}
+  -> int_t t l
 
 
 inline_for_extraction
-val mul_lemma: #t:inttype{t <> U128} -> #l:secrecy_level
-  -> a:uint_t t l
-  -> b:uint_t t l{range (uint_v a `op_Multiply` uint_v b) t}
+val mul_lemma: #t:inttype{t <> U128 /\ t <> S128} -> #l:secrecy_level
+  -> a:int_t t l
+  -> b:int_t t l{range (int_v a `op_Multiply` int_v b) t}
   -> Lemma
-  (ensures (uint_v #t #l (mul #t #l a b) == uint_v a `op_Multiply` uint_v b))
-  [SMTPat (uint_v #t #l (mul #t #l a b))]
+  (ensures (int_v #t #l (mul #t #l a b) == int_v a `op_Multiply` int_v b))
+  [SMTPat (int_v #t #l (mul #t #l a b))]
 
 
 inline_for_extraction
@@ -447,6 +473,15 @@ val mul64_wide_lemma: a:uint64 -> b:uint64
   -> Lemma
   (ensures (uint_v (mul64_wide a b) == uint_v a `op_Multiply` uint_v b))
   [SMTPat (uint_v (mul64_wide a b))]
+
+inline_for_extraction
+val mul_s64_wide: a:int64 -> b:int64 -> int128
+
+inline_for_extraction
+val mul_s64_wide_lemma: a:int64 -> b:int64
+  -> Lemma
+  (ensures (sint_v (mul_s64_wide a b) == sint_v a `op_Multiply` sint_v b))
+  [SMTPat (sint_v (mul_s64_wide a b))]
 
 //inline_for_extraction
 //val mulsigned64_wide: a:int64 -> b:int64 -> int128
@@ -461,42 +496,42 @@ val mul64_wide_lemma: a:uint64 -> b:uint64
 *)
 inline_for_extraction
 val sub_mod: #t:inttype -> #l:secrecy_level
-  -> a:uint_t t l
-  -> b:uint_t t l
-  -> c:uint_t t l
+  -> a:int_t t l
+  -> b:int_t t l
+  -> c:int_t t l
 
 inline_for_extraction
 val sub_mod_lemma: #t:inttype -> #l:secrecy_level ->
-             a:uint_t t l ->
-             b:uint_t t l ->
+             a:int_t t l ->
+             b:int_t t l ->
 	     Lemma
-	     (ensures (uint_v #t #l (sub_mod #t #l a b) == (uint_v a - uint_v b) @%. t))
-	     [SMTPat (uint_v #t #l (sub_mod #t #l a b))]
+	     (ensures (int_v #t #l (sub_mod #t #l a b) == (int_v a - int_v b) @%. t))
+	     [SMTPat (int_v #t #l (sub_mod #t #l a b))]
 
 inline_for_extraction
 val sub: #t:inttype -> #l:secrecy_level
-  -> a:uint_t t l
-  -> b:uint_t t l{range (uint_v a - uint_v b) t}
-  -> uint_t t l
+  -> a:int_t t l
+  -> b:int_t t l{range (int_v a - int_v b) t}
+  -> int_t t l
 
 inline_for_extraction
 val sub_lemma: #t:inttype -> #l:secrecy_level ->
-             a:uint_t t l ->
-             b:uint_t t l{range (uint_v a - uint_v b) t} ->
+             a:int_t t l ->
+             b:int_t t l{range (int_v a - int_v b) t} ->
 	     Lemma
-	     (ensures (uint_v #t #l (sub #t #l a b) == uint_v a - uint_v b))
-	     [SMTPat (uint_v #t #l (sub #t #l a b))]
+	     (ensures (int_v #t #l (sub #t #l a b) == int_v a - int_v b))
+	     [SMTPat (int_v #t #l (sub #t #l a b))]
 
 inline_for_extraction
 val decr: #t:inttype -> #l:secrecy_level
-  -> a:uint_t t l{uint_v a > minint t}
-  -> uint_t t l
+  -> a:int_t t l{int_v a > minint t}
+  -> int_t t l
 
 inline_for_extraction
 val decr_lemma: #t:inttype -> #l:secrecy_level
-  -> a:uint_t t l{uint_v a > minint t}
+  -> a:int_t t l{int_v a > minint t}
   -> Lemma
-  (ensures (uint_v #t #l (decr a) == uint_v a - 1))
+  (ensures (int_v #t #l (decr a) == int_v a - 1))
 
 inline_for_extraction
 let zero (t:inttype) = 0
@@ -509,159 +544,160 @@ inline_for_extraction
 let ones_v (t:inttype) =
   match t with
   | U1 | U8 | U16 | U32 | U64 | U128 -> maxint t
-  | S8 | S16 | S32 | S64 -> -1
+  | S8 | S16 | S32 | S64 | S128 -> -1
 
 
 inline_for_extraction
 val logxor: #t:inttype -> #l:secrecy_level
-  -> a:uint_t t l
-  -> b:uint_t t l
-  -> uint_t t l
+  -> a:int_t t l
+  -> b:int_t t l
+  -> int_t t l
 
-val logxor_lemma: #t:inttype -> a:uint_t t SEC -> b:uint_t t SEC -> Lemma
+val logxor_lemma: #t:inttype -> #l:secrecy_level -> a:int_t t l -> b:int_t t l -> Lemma
   (a `logxor` (a `logxor` b) == b /\
    a `logxor` (b `logxor` a) == b /\
-   a `logxor` (uint #t #SEC 0) == a)
+   a `logxor` (mk_int #t #l 0) == a)
 
-val logxor_lemma1: #t:inttype -> a:uint_t t SEC -> b:uint_t t SEC -> Lemma
+val logxor_lemma1: #t:inttype -> #l:secrecy_level -> a:int_t t l -> b:int_t t l -> Lemma
   (requires range (v a) U1 /\ range (v b) U1)
   (ensures range (v (a `logxor` b)) U1)
 
 inline_for_extraction
 val logand: #t:inttype -> #l:secrecy_level
-  -> a:uint_t t l
-  -> b:uint_t t l
-  -> uint_t t l
+  -> a:int_t t l
+  -> b:int_t t l
+  -> int_t t l
 
-val logand_lemma: #t:inttype{~(U1? t)} -> a:uint_t t SEC -> b:uint_t t SEC -> Lemma
+val logand_lemma: #t:inttype{~(U1? t)} -> a:int_t t SEC -> b:int_t t SEC -> Lemma
   (requires v a = zero t \/ v a = ones_v t)
   (ensures (if v a = zero t then v (a `logand` b) == zero t else v (a `logand` b) == v b))
 
+#reset-options
 let logand_v (#t:inttype{~(U1? t)}) (a: range_t t) (b:range_t t) : range_t t=
 match t with
-  |S8 | S16 | S32 | S64 -> Int.logand #(8*numbytes t) a b
+  |S8 | S16 | S32 | S64 | S128 -> Int.logand #(8*numbytes t) a b
   |_ -> UInt.logand #(8*numbytes t) a b
-  
+
 val logand_spec: #t:inttype{~(U1? t)} -> #l:secrecy_level
-  -> a:uint_t t l -> b:uint_t t l
+  -> a:int_t t l -> b:int_t t l
   -> Lemma (ensures (v (a `logand` b) == (v a `logand_v` v b)))
   //[SMTPat (v (a `logand` b))]
 
 inline_for_extraction
 val logor: #t:inttype -> #l:secrecy_level
-  -> a:uint_t t l
-  -> b:uint_t t l
-  -> uint_t t l
+  -> a:int_t t l
+  -> b:int_t t l
+  -> int_t t l
 
-val logor_disjoint: #t:inttype{(U1? t) \/ (U8? t) \/ (U16? t) \/ (U32? t) \/ (U64? t) \/ (U128? t)} -> a:uint_t t SEC -> b:uint_t t SEC -> m:nat{m < bits t} -> Lemma
+val logor_disjoint: #t:inttype{unsigned t} -> a:int_t t SEC -> b:int_t t SEC -> m:nat{m < bits t} -> Lemma
   (requires 0 <= v a /\ v a < pow2 m /\ v b % pow2 m == 0)
   (ensures v (a `logor` b) == v a + v b)
 
 inline_for_extraction
 val lognot: #t:inttype -> #l:secrecy_level
-  -> a:uint_t t l
-  -> uint_t t l
+  -> a:int_t t l
+  -> int_t t l
 
 inline_for_extraction
-type shiftval (t:inttype) = u:size_t{uint_v u < bits t}
+type shiftval (t:inttype) = u:size_t{int_v u < bits t}
 
 inline_for_extraction
-type rotval  (t:inttype) = u:size_t{uint_v u > 0 /\ uint_v u < bits t}
+type rotval  (t:inttype) = u:size_t{int_v u > 0 /\ int_v u < bits t}
 
 inline_for_extraction
 val shift_right: #t:inttype -> #l:secrecy_level
-  -> a:uint_t t l
+  -> a:int_t t l
   -> b:shiftval t
-  -> c:uint_t t l
+  -> c:int_t t l
 
 val shift_right_lemma: #t:inttype -> #l:secrecy_level
-  -> a:uint_t t l
+  -> a:int_t t l
   -> b:shiftval t
   -> Lemma
-    (ensures uint_v #t #l (shift_right #t #l a b) ==  uint_v #t #l a / pow2 (uint_v #U32 #PUB b))
-    [SMTPat (uint_v #t #l (shift_right #t #l a b))]
+    (ensures int_v #t #l (shift_right #t #l a b) ==  int_v #t #l a / pow2 (int_v #U32 #PUB b))
+    [SMTPat (int_v #t #l (shift_right #t #l a b))]
 
 inline_for_extraction
 val shift_left: #t:inttype -> #l:secrecy_level
-  -> a:uint_t t l
+  -> a:int_t t l
   -> b:shiftval t
-  -> c:uint_t t l
+  -> c:int_t t l
 
 val shift_left_lemma: #t:inttype -> #l:secrecy_level
-  -> a:uint_t t l
+  -> a:int_t t l
   -> b:shiftval t
   -> Lemma
-    (uint_v #t #l (shift_left #t #l a b) == (uint_v #t #l a `op_Multiply` pow2 (uint_v #U32 #PUB b)) @%. t)
-    [SMTPat (uint_v #t #l (shift_left #t #l a b))]
+    (int_v #t #l (shift_left #t #l a b) == (int_v #t #l a `op_Multiply` pow2 (int_v #U32 #PUB b)) @%. t)
+    [SMTPat (int_v #t #l (shift_left #t #l a b))]
 
 inline_for_extraction
 val rotate_right: #t:inttype -> #l:secrecy_level
-  -> a:uint_t t l
+  -> a:int_t t l
   -> b:rotval t
-  -> uint_t t l
+  -> int_t t l
 
 inline_for_extraction
 val rotate_left: #t:inttype -> #l:secrecy_level
-  -> a:uint_t t l
+  -> a:int_t t l
   -> b:rotval t
-  -> uint_t t l
+  -> int_t t l
 
 ///
 /// Masking operators for all machine integers
 ///
 
 inline_for_extraction
-val zeroes: t:inttype -> l:secrecy_level -> v:uint_t t l{uint_v v = zero t}
+val zeroes: t:inttype -> l:secrecy_level -> v:int_t t l{int_v v = zero t}
 
 inline_for_extraction
-val ones: t:inttype -> l:secrecy_level -> v:uint_t t l{uint_v v = ones_v t}
+val ones: t:inttype -> l:secrecy_level -> v:int_t t l{int_v v = ones_v t}
 
 inline_for_extraction
-val eq_mask: #t:inttype{~(S64? t)} -> uint_t t SEC -> uint_t t SEC -> uint_t t SEC
+val eq_mask: #t:inttype{unsigned t} -> int_t t SEC -> int_t t SEC -> int_t t SEC
 
-val eq_mask_lemma: #t:inttype{~(S64? t)} -> a:uint_t t SEC -> b:uint_t t SEC -> Lemma
+val eq_mask_lemma: #t:inttype{unsigned t} -> a:int_t t SEC -> b:int_t t SEC -> Lemma
   (requires True)
   (ensures  (v a = v b ==> v (eq_mask a b) == ones_v t) /\
             (v a <> v b ==> v (eq_mask a b) == 0))
   [SMTPat (eq_mask #t a b)]
 
-val eq_mask_logand_lemma: #t:inttype{~(U1? t) /\ ~(S64? t)} -> a:uint_t t SEC -> b:uint_t t SEC -> c:uint_t t SEC -> Lemma
+val eq_mask_logand_lemma: #t:inttype{unsigned t /\ ~(U1? t)} -> a:int_t t SEC -> b:int_t t SEC -> c:int_t t SEC -> Lemma
   (ensures (if v a = v b then v (c `logand` (eq_mask a b)) == v c else v (c `logand` (eq_mask a b)) == 0))
   [SMTPat (c `logand` (eq_mask a b))]
 
 inline_for_extraction
-val neq_mask: #t:inttype{~(S64? t)} -> a:uint_t t SEC -> b:uint_t t SEC -> uint_t t SEC
+val neq_mask: #t:inttype{unsigned t} -> a:int_t t SEC -> b:int_t t SEC -> int_t t SEC
 
 inline_for_extraction
-val gte_mask: #t:inttype{~(S8? t) /\ ~(S16? t) /\ ~(S32? t) /\ ~(S64? t)} -> uint_t t SEC -> b:uint_t t SEC -> uint_t t SEC
+val gte_mask: #t:inttype{unsigned t} -> int_t t SEC -> b:int_t t SEC -> int_t t SEC
 
-val gte_mask_lemma: #t:inttype{~(S8? t) /\ ~(S16? t) /\ ~(S32? t) /\ ~(S64? t)} -> a:uint_t t SEC -> b:uint_t t SEC -> Lemma
+val gte_mask_lemma: #t:inttype{unsigned t} -> a:int_t t SEC -> b:int_t t SEC -> Lemma
   (requires True)
   (ensures  (v a >= v b ==> v (gte_mask a b) == maxint t) /\
             (v a < v b ==> v (gte_mask a b) == 0))
   [SMTPat (gte_mask #t a b)]
 
-val gte_mask_logand_lemma: #t:inttype{~(U1? t) /\ ~(S8? t) /\ ~(S16? t) /\ ~(S32? t) /\ ~(S64? t)} -> a:uint_t t SEC -> b:uint_t t SEC -> c:uint_t t SEC -> Lemma
+val gte_mask_logand_lemma: #t:inttype{~(U1? t) /\ unsigned t} -> a:int_t t SEC -> b:int_t t SEC -> c:int_t t SEC -> Lemma
   (ensures (if v a >= v b then v (c `logand` (gte_mask a b)) == v c else v (c `logand` (gte_mask a b)) == 0))
   [SMTPat (c `logand` (gte_mask a b))]
 
 inline_for_extraction
-val lt_mask: #t:inttype{~(S8? t) /\ ~(S16? t) /\ ~(S32? t) /\ ~(S64? t)} -> uint_t t SEC -> uint_t t SEC -> uint_t t SEC
+val lt_mask: #t:inttype{unsigned t} -> int_t t SEC -> int_t t SEC -> int_t t SEC
 
 inline_for_extraction
-val gt_mask: #t:inttype{~(S8? t) /\ ~(S16? t) /\ ~(S32? t) /\ ~(S64? t)} -> uint_t t SEC -> b:uint_t t SEC -> uint_t t SEC
+val gt_mask: #t:inttype{unsigned t} -> int_t t SEC -> b:int_t t SEC -> int_t t SEC
 
 inline_for_extraction
-val lte_mask: #t:inttype{~(S8? t) /\ ~(S16? t) /\ ~(S32? t) /\ ~(S64? t)} -> uint_t t SEC -> uint_t t SEC -> uint_t t SEC
+val lte_mask: #t:inttype{unsigned t} -> int_t t SEC -> int_t t SEC -> int_t t SEC
 
 inline_for_extraction
-let mod_mask (#t:inttype{~(S8? t) /\ ~(S16? t) /\ ~(S32? t) /\ ~(S64? t)}) (#l:secrecy_level) (m:shiftval t) : uint_t t l =
-  (nat_to_uint 1 `shift_left` m) `sub_mod` nat_to_uint 1
+let mod_mask (#t:inttype) (#l:secrecy_level) (m:shiftval t) : int_t t l =
+  (nat_to_int 1 `shift_left` m) `sub_mod` nat_to_int 1
 
-val mod_mask_lemma: #t:inttype{~(S8? t) /\ ~(S16? t) /\ ~(S32? t) /\ ~(S64? t)} -> #l:secrecy_level -> a:uint_t t l -> m:shiftval t ->
+val mod_mask_lemma: #t:inttype -> #l:secrecy_level -> a:int_t t l -> m:shiftval t ->
   Lemma
     (requires True)
-    (ensures  uint_v (a `logand` (mod_mask #t m)) == uint_v a % pow2 (uint_v m))
+    (ensures  int_v (a `logand` (mod_mask #t m)) == int_v a % pow2 (int_v m))
     [SMTPat (a `logand` (mod_mask #t m))]
 
 ///
@@ -715,98 +751,101 @@ let ( ~. ) #t #l = lognot #t #l
 ///
 
 inline_for_extraction
-val div: #t:inttype{t <> U128 /\ ~(S8? t) /\ ~(S16? t) /\ ~(S32? t) /\ ~(S64? t)}
-  -> a:uint_t t PUB
-  -> b:uint_t t PUB{uint_v b > 0}
-  -> uint_t t PUB
+val div: #t:inttype{t <> U128 (*/\ t <> S128*) /\ unsigned t}
+  -> a:int_t t PUB
+  -> b:int_t t PUB{int_v b <> 0 (*/\ range (v a / v b) t*)}
+  -> int_t t PUB
 
 inline_for_extraction
-val div_lemma: #t:inttype{t <> U128 /\ ~(S8? t) /\ ~(S16? t) /\ ~(S32? t) /\ ~(S64? t)}
-  -> a:uint_t t PUB
-  -> b:uint_t t PUB{uint_v b > 0}
+val div_lemma: #t:inttype{t <> U128 /\ (*t <> S128*) unsigned t}
+  -> a:int_t t PUB
+  -> b:int_t t PUB{int_v b <> 0 (*/\ range (v a / v b) t*)}
   -> Lemma
-  (ensures (uint_v #t (div #t a b) == uint_v a / uint_v b))
-  [SMTPat (uint_v #t (div #t a b))]
+  (ensures (int_v #t (div #t a b) == int_v a / int_v b))
+  [SMTPat (int_v #t (div #t a b))]
 
 
 inline_for_extraction
-val mod: #t:inttype{t <> U128 /\ ~(S8? t) /\ ~(S16? t) /\ ~(S32? t) /\ ~(S64? t)} -> a:uint_t t PUB -> b:uint_t t PUB{uint_v b > 0} -> uint_t t PUB
+val mod: #t:inttype{t <> U128 (*/\ t <> S128*) /\ unsigned t} 
+  -> a:int_t t PUB 
+  -> b:int_t t PUB{int_v b <> 0 (*/\ range (v a / v b) t*)} 
+  -> int_t t PUB
 
 inline_for_extraction
-val mod_lemma: #t:inttype{t <> U128 /\ ~(S8? t) /\ ~(S16? t) /\ ~(S32? t) /\ ~(S64? t)}
-  -> a:uint_t t PUB
-  -> b:uint_t t PUB{uint_v b > 0}
+val mod_lemma: #t:inttype{t <> U128 /\ (*t <> S128*) unsigned t}
+  -> a:int_t t PUB
+  -> b:int_t t PUB{int_v b <> 0 (*/\ range (v a / v b) t*)}
   -> Lemma
-  (ensures (uint_v #t (mod #t a b) == uint_v a % uint_v b))
-  [SMTPat (uint_v #t (mod #t a b))]
+  (ensures (int_v #t (mod #t a b) == int_v a % int_v b))
+  [SMTPat (int_v #t (mod #t a b))]
 
 
 inline_for_extraction
-val eq: #t:inttype -> uint_t t PUB -> uint_t t PUB -> bool
+val eq: #t:inttype -> int_t t PUB -> int_t t PUB -> bool
 
 inline_for_extraction
 val eq_lemma: #t:inttype
-  -> a:uint_t t PUB
-  -> b:uint_t t PUB
+  -> a:int_t t PUB
+  -> b:int_t t PUB
   -> Lemma
-  (ensures (eq #t a b == (uint_v a = uint_v b)))
+  (ensures (eq #t a b == (int_v a = int_v b)))
   [SMTPat (eq #t a b)]
 
 inline_for_extraction
-val ne: #t:inttype -> uint_t t PUB -> uint_t t PUB -> bool
+val ne: #t:inttype -> int_t t PUB -> int_t t PUB -> bool
 
 inline_for_extraction
 val ne_lemma: #t:inttype
-  -> a:uint_t t PUB
-  -> b:uint_t t PUB
+  -> a:int_t t PUB
+  -> b:int_t t PUB
   -> Lemma
-  (ensures (ne #t a b == (uint_v a <> uint_v b)))
+  (ensures (ne #t a b == (int_v a <> int_v b)))
   [SMTPat (ne #t a b)]
 
 inline_for_extraction
-val lt: #t:inttype -> uint_t t PUB -> uint_t t PUB -> bool
+val lt: #t:inttype -> int_t t PUB -> int_t t PUB -> bool
 
 inline_for_extraction
 val lt_lemma: #t:inttype
-  -> a:uint_t t PUB
-  -> b:uint_t t PUB
+  -> a:int_t t PUB
+  -> b:int_t t PUB
   -> Lemma
-  (ensures (lt #t a b == (uint_v a < uint_v b)))
+  (ensures (lt #t a b == (int_v a < int_v b)))
   [SMTPat (lt #t a b)]
 
 inline_for_extraction
-val lte: #t:inttype -> uint_t t PUB -> uint_t t PUB -> bool
+val lte: #t:inttype -> int_t t PUB -> int_t t PUB -> bool
 
 inline_for_extraction
 val lte_lemma: #t:inttype
-  -> a:uint_t t PUB
-  -> b:uint_t t PUB
+  -> a:int_t t PUB
+  -> b:int_t t PUB
   -> Lemma
-  (ensures (lte #t a b == (uint_v a <= uint_v b)))
+  (ensures (lte #t a b == (int_v a <= int_v b)))
   [SMTPat (lte #t a b)]
 
 
 inline_for_extraction
-val gt: #t:inttype -> uint_t t PUB -> uint_t t PUB -> bool
+val gt: #t:inttype -> int_t t PUB -> int_t t PUB -> bool
 
 inline_for_extraction
 val gt_lemma: #t:inttype
-  -> a:uint_t t PUB
-  -> b:uint_t t PUB
+  -> a:int_t t PUB
+  -> b:int_t t PUB
   -> Lemma
-  (ensures (gt #t a b == (uint_v a > uint_v b)))
+  (ensures (gt #t a b == (int_v a > int_v b)))
   [SMTPat (gt #t a b)]
 
 
 inline_for_extraction
-val gte: #t:inttype -> uint_t t PUB -> uint_t t PUB -> bool
+val gte: #t:inttype -> int_t t PUB -> int_t t PUB -> bool
 
 inline_for_extraction
 val gte_lemma: #t:inttype
-  -> a:uint_t t PUB
-  -> b:uint_t t PUB
+  -> a:int_t t PUB
+  -> b:int_t t PUB
   -> Lemma
-  (ensures (gte #t a b == (uint_v a >= uint_v b)))
+  (ensures (gte #t a b == (int_v a >= int_v b)))
   [SMTPat (gte #t a b)]
 
 inline_for_extraction
